# 2
## a
>$u=\frac12\varepsilon_0E^2+\frac12\frac{B^2}{\mu_0}$
>$u=\frac12\epsilon_0\varepsilon^2\cos^2(kx-\omega t)+\frac12\frac1\mu_0(\frac \varepsilon c)^2\cos^2(kx-\omega t)$
>$u=\frac12\epsilon_0\varepsilon^2\cos^2(kx-\omega t)+\frac12\epsilon_0\varepsilon^2\cos^2(kx-\omega t)$
>$\therefore u=\epsilon_0\varepsilon^2\cos^2(kx-\omega t)$
>$\langle u\rangle=\frac 1T\int_{0}^Tudt$
>$\langle u \rangle=\frac1T\int_0^T\epsilon_0\varepsilon^2\cos^2(kx-\omega t)dt$
>$\therefore\langle u \rangle = \frac12 \epsilon_0\varepsilon^2$
## b
>$\mathbf S=\frac1\mu_0(\mathbf E\times\mathbf B)$
>$\mathbf S=\frac1\mu_0(\varepsilon\cos(kx-\omega t)\hat j\times\frac\varepsilon c\cos(kx-\omega t)\hat k)$
>$\mathbf S=\frac 1 {\mu_0c}\varepsilon^2\cos^2(kx-\omega t)\hat i$
>$c^2=\frac 1 {\mu_0\epsilon_0}\rightarrow c\epsilon_0=\frac 1 {\mu_0c}$
>$\therefore\mathbf S=\epsilon_0 c\varepsilon^2\cos^2(kx-\omega t)\hat i$
>$\langle\mathbf S\rangle=\frac 1 T \int_0^T\mathbf Sdt$
>$\therefore\langle \mathbf S\rangle=\frac {c\epsilon_0\varepsilon^2}2\hat i$
## c
>$\Pi=\frac S {c^2}\rightarrow\therefore\Pi=\frac{\epsilon_0 \varepsilon^2}{c}\cos^2(kx-\omega t)\hat i$
>$\langle \Pi\rangle=\frac 1T\int_0^T\Pi dt$
>$\therefore\langle\Pi\rangle=\frac {\epsilon_0\varepsilon^2}{2c}\hat i$
## d
### i
>$P_{rad}=\frac {\langle S\rangle}c\rightarrow F=PA=\frac {\langle S\rangle A} c$
>$\therefore F=\frac {c\epsilon_0\varepsilon^2}2\hat i\frac Ac=\frac {A\epsilon_0\varepsilon^2}2\hat i$
### ii
>$P_{rad}=\frac {2\langle S\rangle }c\rightarrow F=PA=\frac {2\langle S\rangle A} c$
>$\therefore F=\frac {c\epsilon_0\varepsilon^2}2\hat i\frac {2A}c= {A\epsilon_0\varepsilon^2}\hat i$
## e
### i
>$〈u〉c={\frac J{m^3}}{\frac ms}=\frac J {m^2s}$
>$〈u〉/c=\frac {\frac J{m^3}}{m/s}=\frac {Js} {m^4}$
>$I=\frac W{m^2}=\frac J{m^2s}$ from question f
>$\therefore I=\langle u\rangle c$
### ii
>$〈u〉/c=\frac {\frac J{m^3}}{m/s}=\frac {Js} {m^4}$
>$〈u〉c={\frac J{m^3}}{\frac ms}=\frac J {m^2s}$
>$J=\frac {kg m^2}{s^2}$
>$〈u〉c=\frac {kg}{s^3}, 〈u〉/c=\frac {kg}{m^2s}$
>$\langle\Pi\rangle=\frac{kg}{m^2s}$ from question f iii
>$\therefore\langle\Pi\rangle=\langle u\rangle/c$
## f
>$I=1360 \frac W{m^2}$
### i

>$1360=\frac {c\epsilon_0\varepsilon^2}2\hat i$
>$\therefore\varepsilon=\sqrt{\frac{2*1360}{(3.0\times10^8)(8.85\times10^{-12})}}=1012.17 \frac Vm$
>$\therefore\frac\varepsilon c=\frac {1012.17}{3.0\times10^8}=3.37\times10^{-6}T$
### ii
>$1360=\langle u \rangle c\rightarrow \langle u \rangle=\frac {1360}c$
> $\therefore\langle u \rangle = 4.53\times10^{-6}\frac J{m^3}$
### iii
>$\langle\Pi\rangle=\langle u\rangle/c=\frac{4.53\times10^{-6}}{3.0\times10^8}$
>$\therefore\langle\Pi\rangle=1.51\times10^{-14}\frac{kg}{m^2s}$
### iv
>$1 mi^2= 2.59\times10^6m^2$
>$F=A\epsilon_0\varepsilon^2$ from d
>$\therefore F=(2.59\times10^6)(8.85\times10^{-12})(1012.17)^2=23.48N$
# 4
## a
>$I=\frac W{m^2}\rightarrow I=\frac LA$
>$\therefore I=\frac L{4\pi R^2}$
## b
>$F=\frac {IA}c$
>$A=$ Cross Section Area
>$A=\pi r^2$
>$F=\frac {L\pi r^2}{4\pi R^2c}$
>$\therefore F=\frac{Lr^2}{4R^2c}$
## c
>$F=G\frac {m_1m_2}{R^2}-\frac{IA}c=0$
>$G\frac {M\rho \frac43 \pi r^3}{R^2}=\frac {Lr^2}{4R^2c}$
>$\therefore r=\frac {3L}{16cMG\rho \pi}$ meters
## d
>$r=\frac{3L}{16cMG\rho \pi}\rightarrow r=\frac{(3)(4\times10^{26} W)}{(16\pi)(3\times10^8\frac ms)(2\times10^{30} kg)(6.67\times10^{-11}\frac{Nm^2}{kg^2})(2.5\times10^{3}\frac {kg}{m^3})}$
>$\therefore r= 2.386\times10^-7\frac{Ws}{N}=2.386\times10^-7\frac{Nm}{s}\frac sN=2.386\times10^-7m$
# 5
## a
>$\oint \vec B \cdot d\vec s=\mu_0I_{enc} + \mu_0\varepsilon_0\frac{d\Phi_E}{dt}$
>$\Phi_E=\oint\vec E\cdot d\vec a$
>$\Phi_E=\vec E\oint d\vec a$
>$\Phi_E=E_0\sin(\omega t)\hat i (2\pi R^2)$
>$\frac{d\Phi_E}{dt}=E_0\cos(\omega t)(2\pi R^2)\hat i$
>$\vec B\oint d\vec s=\mu_0(I_{enc}+\varepsilon_0E_0\cos(\omega t)(2\pi R^2)\hat i)$
>$\vec B\oint d\vec s=\mu_0\varepsilon_0E_0\cos(\omega t)(2\pi R^2)\hat i$
>$\vec B 2\pi R=\mu_0\varepsilon_0E_0\cos(\omega t)(2\pi R^2)\hat i$
>$\vec B = \mu_0\varepsilon_0E_0R\cos(\omega t)$ Counter Clockwise
## b
>$\vec B 2\pi (2R)=\mu_0\varepsilon_0E_0\cos(\omega t)(2\pi (2R)^2)$
>$\vec B = 2\mu_0\varepsilon_0E_0R\cos(\omega t)$ Counter Clockwise